lean/Nucleus/Nucleus/Hol/Propane.lean
@@ -1,5 +1,6 @@
 import Nucleus.Hol.Propane.Semantics
 import Nucleus.Hol.Propane.Table.Nat
 import Nucleus.Hol.Propane.Compact
+import Nucleus.Hol.Propane.Ethane
 
 /-! # Propane: the always-well-typed HOL experiment -/
